# Latex



$\begin{equation}
a^2 + b^2 = c^2 \tag{1.1}
\end{equation}$



$$\lim_{n \to \infty}
\sum_{k=1}^n \frac{1}{k^2}
= \frac{\pi^2}{6}$$.

$$
\lim_{n \to \infty}
\sum_{k=1}^n \frac{1}{k^2}
= \frac{\pi^2}{6}
$$


$$x^{2} \geq 0 \qquad \text{for all} \: x\in\mathbb{R}$$


$$a_1, a_2, \dots, a_n$$



$$a_1 + a_2 + \cdots + a_n$$



$$p^3_{ij} \qquad m_\mathrm{Knuth}\qquad \sum_{k=1}^3 k $$  



$$a^x+y \neq a^{x+y}\qquad e^{x^2} \neq {e^x}^2$$



$$f(x) = x^2 \quad f'(x) = 2x \quad f''^{2}(x) = 4$$



$$
3/8 \qquad \frac{3}{8} \qquad \tfrac{3}{8}
$$



$$1\frac{1}{2}$$ hours $$\qquad 1\dfrac{1}{2}$$hours



$$\sqrt{x} \Leftrightarrow x^{1/2} \quad \sqrt[3]{2} \quad \sqrt{x^{2} + \sqrt{y}}$$



$$
\binom{n}{k} =\binom{n-1}{k} + \binom{n-1}{k-1}
$$



$$f_n(x) \stackrel{*}{\approx} 1$$



$$ \lim_{x \rightarrow 0} \frac{\sin x}{x}=1 $$



$$ a\bmod b \\ x\equiv a \pmod{b} $$



$$\sum_{i=1}^n \quad \int_0^{\frac{\pi}{2}} \quad \oint_0^{\pi / 2 } \quad \prod_\epsilon $$



$$\sum_{i=1}^n \quad \int_0^{\frac{\pi}{2}} \quad \oint_0^{\pi / 2 } \quad \prod_\epsilon $$



$$\sum\limits_{i=1}^n \quad \int\limits_0^{\frac{\pi}{2}} \quad \prod\limits_\epsilon $$



$$\sum\nolimits_{i=1}^n \quad \int\limits_0^{\frac{\pi}{2}} \quad \prod\nolimits_\epsilon$$



$$\sum_{\substack{0\le i\le n \\
j\in \mathbb{R}}} P(i,j) = Q(n)$$



$$\sum_{\begin{subarray}{l} 0\le i\le n \\
j\in \mathbb{R} \end{subarray}} P(i,j) = Q(n)$$



$$\bar{x_0} \quad \bar{x}_0$$



$$\vec{x_0} \quad \vec{x}_0$$



$$\hat{\mathbf{e}_x} \quad \hat{\mathbf{e}}_x$$



$$0.\overline{3} = \underline{\underline{1/3}}$$



$$1 + \left(\frac{1}{1-x^{2}} \right)^3 \qquad \left.\frac{\partial f}{\partial t} \right|_{t=0}$$



$$\Bigl((x+1)(x-1)\Bigr)^{2}$$  



$${a,b,c} \neq \{a,b,c\}$$



$$\bigl( \Bigl( \biggl( \Biggl( \quad
\bigr\} \Bigr\} \biggr\} \Biggr\} \quad
\big\| \Big\| \bigg\| \Bigg\| \quad
\big\Downarrow \Big\Downarrow
\bigg\Downarrow \Bigg\Downarrow$$



$$
\begin{multline}
a + b + c + d + e + f

+ g + h + i \\
  = j + k + l + m + n\\
  = o + p + q + r + s\\
  = t + u + v + x + z
  \end{multline}
$$

$$
\begin{align}
a & = b + c \\
& = d + e
\end{align}
$$

$$
\begin{align}
a ={} & b + c \\
={} & d + e + f + g + h + i

+ j + k + l  \\
  & + m + n + o \\
  ={} & p + q + r + s
  \end{align}
$$



$$
\begin{align}
a &=1 & b &=2 & c &=3 \\
d &=-1 & e &=-2 & f &=-5
\end{align}
$$

$$
\begin{align}
a = b + c \\
d = e + f + g \\
h + i = j + k  \\
l + m = n
\end{align}
$$
$$
\begin{gather}
a = b + c \\
d = e + f + g \\
h + i = j + k  \\
l + m = n
\end{gather}
$$
$$
\begin{equation}
\begin{aligned}
a &= b + c \\
d &= e + f + g \\
h + i &= j + k \\
l + m &= n
\end{aligned} \tag{1.3}
\end{equation}
$$


$$
 \mathbf{X} = \left(
\begin{array}{cccc}
x_{11} & x_{12} & \ldots & x_{1n}\\
x_{21} & x_{22} & \ldots & x_{2n}\\
\vdots & \vdots & \ddots & \vdots\\
x_{n1} & x_{n2} & \ldots & x_{nn}\\
\end{array} \right)
$$



$$
 |x| = \left\{
\begin{array}{rl}
-x & \text{if } x < 0,\\
0 & \text{if } x = 0,\\
x & \text{if } x > 0.
\end{array} \right. 
$$



$$
|x| = \begin{cases}
-x & \text{if } x < 0,\\
0 & \text{if } x = 0,\\
x & \text{if } x > 0.
\end{cases}
$$



$$
\begin{matrix} 1 & 2 \\
3 & 4 \end{matrix}
$$
$$

\begin{pmatrix} 1 & 2 \\
3 & 4 \end{pmatrix} 
$$
$$
\begin{bmatrix}
x_{11} & x_{12} & \ldots & x_{1n}\\
x_{21} & x_{22} & \ldots & x_{2n}\\
\vdots & \vdots & \ddots & \vdots\\
x_{n1} & x_{n2} & \ldots & x_{nn}\\
\end{bmatrix}
$$



$$\mathcal{R} \quad \mathfrak{R} \quad \mathbb{R}$$
$$\mathcal{L} = -\frac{1}{4}F_{\mu\nu}F^{\mu\nu}$$
$$\mathfrak{su}(2)$$ and $$\mathfrak{so}(3)$$ Lie algebra



$$\mu, M \qquad \boldsymbol{\mu}, \boldsymbol{M}$$



$$
r = \frac
{\sum_{i=1}^n (x_i- x)(y_i- y)}
{\displaystyle \left[
\sum_{i=1}^n (x_i-x)^2
\sum_{i=1}^n (y_i-y)^2
\right]^{1/2} }
$$



$$\because a \ge b \\ b \ge c \\ \therefore a \ge c$$


$$
\begin{align}
\because a \ge b \\ b \ge c \\ \therefore a \ge c
\end{align}
$$
